src/impl/TLS13.Impl.ConnectionState.Model.fst
@@ -439,6 +439,7 @@ let lemma_client_handshake_traffic_install_legal
   : Lemma
       (requires model.CS.model_control ==
                   CS.ControlHandshaking CS.HsServerHelloReceived /\
+                model.CS.model_config.CS.config_role == CS.ClientEndpoint /\
                 model.CS.model_handshake.CS.hs_keys.CS.ks_handshake_secret ==
                   Some handshake_secret)
       (ensures CS.legal_event
@@ -462,6 +463,7 @@ let lemma_server_handshake_traffic_install_legal
   : Lemma
       (requires model.CS.model_control ==
                   CS.ControlHandshaking CS.HsServerHelloReceived /\
+                model.CS.model_config.CS.config_role == CS.ClientEndpoint /\
                 model.CS.model_handshake.CS.hs_keys.CS.ks_handshake_secret ==
                   Some handshake_secret)
       (ensures CS.legal_event
@@ -485,6 +487,7 @@ let lemma_client_application_traffic_install_legal
   : Lemma
       (requires model.CS.model_control ==
                   CS.ControlHandshaking CS.HsServerFinishedVerified /\
+                model.CS.model_config.CS.config_role == CS.ClientEndpoint /\
                 model.CS.model_handshake.CS.hs_keys.CS.ks_master_secret ==
                   Some master_secret)
       (ensures CS.legal_event
@@ -508,6 +511,7 @@ let lemma_server_application_traffic_install_legal
   : Lemma
       (requires model.CS.model_control ==
                   CS.ControlHandshaking CS.HsServerFinishedVerified /\
+                model.CS.model_config.CS.config_role == CS.ClientEndpoint /\
                 model.CS.model_handshake.CS.hs_keys.CS.ks_master_secret ==
                   Some master_secret)
       (ensures CS.legal_event
@@ -532,6 +536,8 @@ let lemma_received_hello_retry_request_rejected_state_evolves
       (requires CS.connection_state_consistent st /\
                 st.CS.cs_model.CS.model_control ==
                   CS.ControlHandshaking CS.HsClientHelloSent /\
+                st.CS.cs_model.CS.model_config.CS.config_role ==
+                  CS.ClientEndpoint /\
                 CS.event_raw_delta_legal
                   st.CS.cs_model
                   (CS.ConnNetworkEvent {
@@ -720,6 +726,8 @@ let lemma_received_encrypted_extensions_state_evolves
       (requires CS.connection_state_consistent st /\
                 st.CS.cs_model.CS.model_control ==
                   CS.ControlHandshaking CS.HsServerHelloReceived /\
+                st.CS.cs_model.CS.model_config.CS.config_role ==
+                  CS.ClientEndpoint /\
                 Some?
                   st.CS.cs_model.CS.model_handshake.CS.hs_keys.CS.ks_server_handshake_traffic /\
                 CS.event_raw_delta_legal
@@ -786,6 +794,8 @@ let lemma_received_certificate_state_evolves
       (requires CS.connection_state_consistent st /\
                 st.CS.cs_model.CS.model_control ==
                   CS.ControlHandshaking CS.HsEncryptedExtensionsReceived /\
+                st.CS.cs_model.CS.model_config.CS.config_role ==
+                  CS.ClientEndpoint /\
                 cert.M.chain <> [] /\
                 CS.event_raw_delta_legal
                   st.CS.cs_model
@@ -851,6 +861,8 @@ let lemma_received_certificate_verify_state_evolves
       (requires CS.connection_state_consistent st /\
                 st.CS.cs_model.CS.model_control ==
                   CS.ControlHandshaking CS.HsCertificateValidated /\
+                st.CS.cs_model.CS.model_config.CS.config_role ==
+                  CS.ClientEndpoint /\
                 Some?
                   st.CS.cs_model.CS.model_handshake.CS.hs_validated_peer /\
                 CS.event_raw_delta_legal
@@ -960,6 +972,8 @@ let lemma_received_server_finished_state_evolves
       (requires CS.connection_state_consistent st /\
                 st.CS.cs_model.CS.model_control ==
                   CS.ControlHandshaking CS.HsCertificateVerifyVerified /\
+                st.CS.cs_model.CS.model_config.CS.config_role ==
+                  CS.ClientEndpoint /\
       Some?
         st.CS.cs_model.CS.model_handshake.CS.hs_keys.CS.ks_server_handshake_traffic /\
       CS.event_raw_delta_legal
@@ -1163,6 +1177,8 @@ let lemma_received_close_notify_state_evolves
       (requires CS.connection_state_consistent st /\
                 (st.CS.cs_model.CS.model_control == CS.ControlApplicationData \/
                  st.CS.cs_model.CS.model_control == CS.ControlClosing) /\
+                st.CS.cs_model.CS.model_config.CS.config_role ==
+                  CS.ClientEndpoint /\
                 CS.event_raw_delta_legal
                   st.CS.cs_model
                   (CS.ConnNetworkEvent {
@@ -1281,6 +1297,8 @@ let lemma_received_application_data_state_evolves
   : Lemma
       (requires CS.connection_state_consistent st /\
                 st.CS.cs_model.CS.model_control == CS.ControlApplicationData /\
+                st.CS.cs_model.CS.model_config.CS.config_role ==
+                  CS.ClientEndpoint /\
                 Some? st.CS.cs_model.CS.model_handshake.CS.hs_keys.CS.ks_server_application_traffic /\
                 CS.event_raw_delta_legal
                   st.CS.cs_model
@@ -1345,6 +1363,8 @@ let lemma_received_ignored_post_handshake_state_evolves
   : Lemma
       (requires CS.connection_state_consistent st /\
                 st.CS.cs_model.CS.model_control == CS.ControlApplicationData /\
+                st.CS.cs_model.CS.model_config.CS.config_role ==
+                  CS.ClientEndpoint /\
                 Some? st.CS.cs_model.CS.model_handshake.CS.hs_keys.CS.ks_server_application_traffic /\
                 CS.event_raw_delta_legal
                   st.CS.cs_model
@@ -1409,6 +1429,8 @@ let lemma_received_key_update_state_evolves
   : Lemma
       (requires CS.connection_state_consistent st /\
                 st.CS.cs_model.CS.model_control == CS.ControlApplicationData /\
+                st.CS.cs_model.CS.model_config.CS.config_role ==
+                  CS.ClientEndpoint /\
                 Some? st.CS.cs_model.CS.model_handshake.CS.hs_keys.CS.ks_server_application_traffic /\
                 CS.event_raw_delta_legal
                   st.CS.cs_model
@@ -1472,6 +1494,8 @@ let lemma_received_key_update_not_requested_state_evolves
   : Lemma
       (requires CS.connection_state_consistent st /\
                 st.CS.cs_model.CS.model_control == CS.ControlApplicationData /\
+                st.CS.cs_model.CS.model_config.CS.config_role ==
+                  CS.ClientEndpoint /\
                 Some? st.CS.cs_model.CS.model_handshake.CS.hs_keys.CS.ks_server_application_traffic /\
                 CS.event_raw_delta_legal
                   st.CS.cs_model
